Make wsat store interpretation instead of formula

nola/examples/aprop.v
@@ -1,5 +1,4 @@
 From nola.iris Require Import cif inv sinv.
-From nola.iris Require Export inv_deriv.
 From nola.bi Require Import deriv.
 From nola.util Require Import tagged.
 From iris.base_logic.lib Require Export wsat invariants.
@@ -20,8 +19,8 @@ Section embedding.
   | IProp :
     ∀ (P : iProp Σ), aProp true
   | FProp :
-    ∀ (P : (JUDG -n> iProp Σ) -> iProp Σ) (P_cif : cif CON Σ),
-      (∀ δ, ⟦ P_cif ⟧ᶜ(δ) ∗-∗ P δ) ->
+    ∀ (P : iProp Σ) (P_cif : cif CON Σ),
+      (⟦ P_cif ⟧ᶜ ∗-∗ P) ->
       aProp false.
 
   (** We need to parameterise [P] in [FProp P P_cif Hiff] because
@@ -46,22 +45,22 @@ Section embedding.
 
   Definition nola_prop := aProp false.
   Definition iris_prop := aProp true.
-  Definition aProp_to_iProp_deriv δ {b} (P: aProp b) :=
+  Definition aProp_to_iProp_deriv {b} (P: aProp b) :=
   match P with
   | IProp P => P
-  | FProp P _ _ => P δ
+  | FProp P _ _ => P
   end.
 
   Program Definition IProp_to_FProp {b} (P : aProp b) : aProp false :=
     match P with
-    | IProp P => FProp (λ _, ▷ P)%I (▷ P)%cif _
+    | IProp P => FProp (▷ P)%I (▷ P)%cif _
     | FProp iP P HP => FProp iP P HP
     end.
 
   Coercion aProp_to_bi_car {b} (P : aProp b) : bi_car (iProp Σ) :=
     match P with
     | IProp P => P
-    | FProp iP P HP => iP der
+    | FProp iP P HP => iP
     end.
 
   Program Definition nola_to_FML (P : aProp false) : cif CON Σ.
@@ -70,10 +69,10 @@ Section embedding.
     apply P_cif.
   Defined.
 
-  Lemma sm_to_FML (P : aProp false) : ⟦ nola_to_FML P ⟧ᶜ ≡ aProp_to_iProp_deriv der P.
+  Lemma sm_to_FML (P : aProp false) : ⟦ nola_to_FML P ⟧ᶜ ≡ aProp_to_iProp_deriv P.
   Proof.
     dependent destruction P; cbn.
-    iSplit; by [ iPoseProof (b der) as "[Himp _]" |iPoseProof (b der) as "[_ Himp]" ].
+    iSplit; by [ iPoseProof b as "[Himp _]" |iPoseProof b as "[_ Himp]" ].
   Qed.
 
   Coercion aProp_to_FML {b} : aProp b -> cif CON Σ :=
@@ -84,7 +83,7 @@ Section embedding.
 
   Definition ofe_car_iprop := ofe_car (iProp Σ).
   Coercion aProp_to_ofe_car' {b} (P : aProp b) : ofe_car_iprop
-    := aProp_to_iProp_deriv der P.
+    := aProp_to_iProp_deriv P.
 
   Definition ofe_car_ofunc {CON Σ} := ofe_car (oFunctor_apply (cifOF CON) (iProp Σ)).
   Coercion aProp_to_ofe_car_func {b} (P : aProp b) : ofe_car_ofunc
@@ -92,17 +91,16 @@ Section embedding.
 
 End embedding.
 
-Arguments aProp _ _ _ {_} _.
+Arguments aProp _ _ _ {_ _}.
 
-Notation "↑⟦ P ⟧" := (aProp_to_iProp_deriv der P).
-Notation "↑⟦ P ⟧( δ )" := (aProp_to_iProp_deriv δ P).
+Notation "↑⟦ P ⟧" := (aProp_to_iProp_deriv P).
 
 Record NotDeriv `{!Csem CON JUDG Σ} `{!Jsem JUDG (iProp Σ)}
   {b} (p : aProp CON JUDG Σ b) := NOT_DERIV {
     not_deriv : match p with
     | IProp _ => True
     | FProp iP P HP =>
-      ∃ Q, ∀ δ, iP δ ∗-∗ Q
+      ∃ Q, iP ∗-∗ Q
     end;
   }.
 
@@ -115,32 +113,23 @@ Section connectives.
   Local Notation "'aProp'" := (aProp CON JUDG Σ).
 
   Definition aProp_equivalence {b₁ b₂} (P : aProp b₁) (Q : aProp b₂) : iProp Σ :=
-    ⌜b₁ = b₂⌝ ∗ (∀ δ ih, ⌜Deriv ih δ⌝ -∗ ↑⟦ P ⟧(δ) ∗-∗ ↑⟦ Q ⟧(δ)).
-
-  (* Lemma aProp_equiv' b1 : Equivalence (@aProp_equivalence b1).
-  Proof.
-    split.
-    - intros P δ.
-      apply bi.wand_iff_refl.
-    - intros P Q Hequiv δ. specialize (Hequiv δ).
-      by iApply util.wand_iff_comm.
-    - intros P Q R HPQ HQR δ.
-      iApply bi.wand_iff_trans. iSplitL.
-      + iApply (HPQ δ).
-      + iApply (HQR δ).
-  Qed. *)
+    match P, Q with
+    | IProp P, IProp Q => P ∗-∗ Q
+    | IProp P, FProp iQ _ _ => ▷ P ∗-∗ iQ
+    | FProp iP _ _, IProp Q => iP ∗-∗ ▷ Q
+    | FProp iP _ _, FProp iQ _ _ => iP ∗-∗ iQ
+    end.
 
   Program Definition aProp_sep {b₁ b₂ : bool} (P : aProp b₁) (Q : aProp b₂) : aProp (b₁ || b₂) :=
     match P, Q with
     | IProp P, IProp Q => IProp (P ∗ Q)%I
-    | IProp P, FProp Q _ _ => IProp (P ∗ Q der)%I
-    | FProp P _ _, IProp Q => IProp (P der ∗ Q)%I
+    | IProp P, FProp Q _ _ => IProp (P ∗ Q)%I
+    | FProp P _ _, IProp Q => IProp (P ∗ Q)%I
     | FProp iP P HP, FProp iQ Q HQ =>
-        FProp (λ δ, iP δ ∗ iQ δ)%I (P ∗ Q)%cif _
+        FProp (iP ∗ iQ)%I (P ∗ Q)%cif _
     end.
   Next Obligation.
     clear Heq_P Heq_Q.
-    specialize (HP δ); specialize (HQ δ).
     iSplit;
       by (iIntros "[HP HQ]";
        iSplitL "HP";
@@ -153,7 +142,7 @@ Section connectives.
     dependent destruction P; dependent destruction Q; cbn; try done.
     destruct NotDeriv0 as [[Qp HP]]. destruct NotDeriv1 as [[Qq HQ]].
     constructor. exists (Qp ∗ Qq)%I.
-    intros δ. iSplit; iIntros "[HP HQ]";
+    iSplit; iIntros "[HP HQ]";
       (iSplitL "HP"; [ iApply HP; iApply "HP" | iApply HQ; iApply "HQ" ]).
   Qed.
 
@@ -162,8 +151,8 @@ Section connectives.
     destruct b.
     - constructor.
       refine (∀ a, ↑⟦ P a ⟧)%I.
-    - eapply (FProp (λ δ, ∀ a, ↑⟦ P a ⟧(δ))%I (∀ a, aProp_to_FML (P a))%cif).
-      intros δ. simpl.
+    - eapply (FProp (∀ a, ↑⟦ P a ⟧)%I (∀ a, aProp_to_FML (P a))%cif).
+      simpl.
       iSplit; iIntros "HP %a"; iSpecialize ("HP" $! a);
         remember (P a) as Q; dependent destruction Q; cbn;
         by iApply b.
@@ -180,8 +169,8 @@ Section connectives.
     destruct b.
     - constructor.
       refine (∃ a, ↑⟦ P a ⟧)%I.
-    - eapply (FProp (λ δ, ∃ a, ↑⟦ P a ⟧(δ))%I (∃ a, aProp_to_FML (P a))%cif).
-      intros δ; simpl.
+    - eapply (FProp (∃ a, ↑⟦ P a ⟧)%I (∃ a, aProp_to_FML (P a))%cif).
+      simpl.
       iSplit; iIntros "[%a HP]"; iExists a;
         remember (P a) as Q; dependent destruction Q; cbn;
         by iApply b.
@@ -196,14 +185,13 @@ Section connectives.
   Program Definition aProp_wand {b₁ b₂ : bool} (P : aProp b₁) (Q : aProp b₂) : aProp (b₁ || b₂) :=
     match P, Q with
     | IProp P, IProp Q => IProp (P -∗ Q)%I
-    | IProp P, FProp Q _ _ => IProp (P -∗ Q der)%I
-    | FProp P _ _, IProp Q => IProp (P der -∗ Q)%I
+    | IProp P, FProp Q _ _ => IProp (P -∗ Q)%I
+    | FProp P _ _, IProp Q => IProp (P -∗ Q)%I
     | FProp iP P HP, FProp iQ Q HQ =>
-        FProp (λ δ, iP δ -∗ iQ δ)%I (P -∗ Q)%cif _
+        FProp (iP -∗ iQ)%I (P -∗ Q)%cif _
     end.
   Next Obligation.
     clear Heq_P Heq_Q.
-    specialize (HP δ); specialize (HQ δ).
     iSplit; iIntros "HP→Q HP"; iApply HQ; iApply "HP→Q".
     - iPoseProof HP as "[_ HiP→P]"; by iApply "HiP→P".
     - iPoseProof HP as "[HP→iP _]"; by iApply "HP→iP".
@@ -215,17 +203,17 @@ Section connectives.
     dependent destruction P; dependent destruction Q; cbn; try done.
     destruct NotDeriv0 as [[Qp HP]]. destruct NotDeriv1 as [[Qq HQ]].
     constructor. exists (Qp -∗ Qq)%I.
-    intros δ. iSplit; iIntros "Himp HP";
+    iSplit; iIntros "Himp HP";
       iApply HQ; iApply "Himp"; iApply HP; iApply "HP".
   Qed.
 
   Program Definition aProp_pure (P : Prop) : aProp false :=
-    FProp (λ _, ⌜P⌝%I) (cif_pure P) _.
+    FProp (⌜P⌝%I) (cif_pure P) _.
 
   #[export] Instance notderiv_pure P : NotDeriv (aProp_pure P).
   Proof.
     constructor;cbn.
-    exists (⌜ P ⌝)%I. intros _.
+    exists (⌜ P ⌝)%I.
     apply bi.wand_iff_refl.
   Qed.
 
@@ -245,13 +233,12 @@ From nola.examples Require Import con deriv.
 Section inv.
 
   Context `{!Csem CON JUDG Σ, !Jsem JUDG (iProp Σ), !lrustGS_gen hlc Σ,
-    !inv'GS (cifOF CON) Σ, !invC CON, !iffJ (cifO CON Σ) JUDG,
-    !invCS CON JUDG Σ, !iffJS (cifOF CON) JUDG Σ}.
+    !inv'GS Σ, !inv_tokC CON, !inv_tokCS CON JUDG Σ}.
 
   Local Notation "'aProp'" := (aProp CON JUDG Σ).
 
   Program Definition ainv_tok {b} N (P : aProp b) : aProp false :=
-    FProp (λ δ, inv' δ N P) (cif_inv N P) _.
+    FProp (inv_tok N P) (cif_inv_tok N P) _.
   Next Obligation.
     unfold aProp_to_ofe_car, aProp_to_FML; simpl.
     setoid_rewrite sem_cif_in; simpl.
@@ -259,35 +246,14 @@ Section inv.
   Defined.
   Arguments ainv_tok {_} _ _%_aprop_scope.
 
-  (** Allocate [inv_tok] suspending the world satisfaction *)
-  Lemma inv'_tok_alloc_suspend {sm} Px N :
-    inv_wsat sm ==∗ invd N Px ∗ (sm Px -∗ inv_wsat sm).
-  Proof.
-    rewrite /inv' inv.inv_wsat_unseal. iIntros "W".
-    iDestruct (sinv_tok_alloc_suspend Px with "W") as (I) "big".
-    iMod (alloc_ownD I N) as (???) "D". iMod ("big" with "[//]") as "[#i →W]".
-    iModIntro. iSplitR.
-    { iExists Px. rewrite inv.inv_tok_unseal. iFrame "i %".
-      iApply Deriv_factor; iIntros.
-      rewrite in_js. cbn. unfold iffJT_sem. iModIntro.
-      iSplit; by iIntros. }
-    iIntros "HP". iApply "→W". unfold inv.inv_sem. iLeft. iFrame.
-  Qed.
-  (** Allocate [inv_tok] *)
-  Lemma inv'_tok_alloc {sm} Px N : sm Px =[inv_wsat sm]=∗ invd N Px.
-  Proof.
-    iIntros "? W". iMod (inv'_tok_alloc_suspend with "W") as "[$ →W]". iModIntro.
-    by iApply "→W".
-  Qed.
-
   Definition invariant_unfold {b} (P : aProp b) := IProp_to_FProp P.
 
   Lemma ainv_tok_alloc {b} N (P : aProp b) :
-    P -∗ bupdw (inv_wsat ⟦⟧ᶜ) (ainv_tok N P).
+    P -∗ bupdw (inv_wsat) (ainv_tok N P).
   Proof.
     iIntros "HP W".
     unfold ainv_tok. simpl.
-    iMod ( @inv'_alloc CON JUDG Σ Csem0 Jsem0 hlc _ _ _ _ _ _ der_Deriv with "[HP] W") as "[W Hinv]".
+    iMod (inv_tok_alloc with "[HP] W") as "[W Hinv]".
     { instantiate (1 := P).
       dependent destruction P; cbn.
       - iApply "HP".
@@ -297,7 +263,7 @@ Section inv.
   Qed.
 
   Lemma ainv_tok_inv_alloc {b} N1 N2 (P : aProp b) : N1 ## N2 ->
-    P -∗ bupdw (inv_wsat ⟦⟧ᶜ) (ainv_tok N2 (ainv_tok N1 P)).
+    P -∗ bupdw (inv_wsat) (ainv_tok N2 (ainv_tok N1 P)).
   Proof.
     iIntros (Hmasks) "HP W".
     iMod (ainv_tok_alloc with "HP W") as "[W #Hinv]".
@@ -307,35 +273,21 @@ Section inv.
   Qed.
 
   Lemma ainv_tok_acc {N E b} {Px : aProp b} : ↑N ⊆ E →
-    ainv_tok N Px =[inv_wsat ⟦⟧ᶜ]{E,E∖↑N}=∗
-      (invariant_unfold Px) ∗ (invariant_unfold Px =[inv_wsat ⟦⟧ᶜ]{E∖↑N,E}=∗ True).
+    ainv_tok N Px =[inv_wsat]{E,E∖↑N}=∗
+      (invariant_unfold Px) ∗ (invariant_unfold Px =[inv_wsat]{E∖↑N,E}=∗ True).
   Proof.
-    simpl.
-    rewrite /inv' inv.inv_wsat_unseal => NE. iIntros "[%Q #[HJ sm]] W".
-    iDestruct (der_sound with "HJ") as "{HJ}HJ"; rewrite in_js /= /iffJT_sem.
-    rewrite inv.inv_tok_unseal; iDestruct "sm" as "(%i & %iN & sm)".
-    iMod (inv.fupd_ownE_acc_in iN NE) as "[i cl]".
-    iDestruct (sinv_tok_acc with "sm W") as "[in →W]".
-    iDestruct "in" as "[[HP D]|i']"; last first.
-    { iDestruct (ownE_singleton_twice with "[$i $i']") as %[]. }
-    iDestruct ("→W" with "[$i]") as "$". iIntros "!>".
-    iSplitL "HP".
-    { dependent destruction Px; cbn.
-      - by iApply "HJ".
-      - iApply b. by iApply "HJ". }
-    iIntros "Px W".
-    iDestruct (sinv_tok_acc with "sm W") as "[[[_ D']|i] →W]".
-    { iDestruct (ownD_singleton_twice with "[$D $D']") as %[]. }
-    iMod ("cl" with "i") as "_". iModIntro. iSplit; [|done]. iApply "→W".
-    iLeft. iFrame.
+    intros HNE.
     dependent destruction Px; cbn.
-    - iApply ("HJ" with "Px").
-    - iApply "HJ". by iApply b.
+    - apply (inv.inv_tok_acc HNE (Px := ▷ P)).
+    - iIntros "Hinv W".
+      apply bi.wand_iff_equiv in b.
+      rewrite <- b.
+      iApply (inv.inv_tok_acc HNE with "Hinv W").
   Qed.
 
   Lemma ainv_tok_acc_nola {N E} {Px : aProp false} : ↑N ⊆ E →
-    ainv_tok N Px =[inv_wsat ⟦⟧ᶜ]{E,E∖↑N}=∗
-      Px ∗ (Px =[inv_wsat ⟦⟧ᶜ]{E∖↑N,E}=∗ True).
+    ainv_tok N Px =[inv_wsat]{E,E∖↑N}=∗
+      Px ∗ (Px =[inv_wsat]{E∖↑N,E}=∗ True).
   Proof.
     iIntros (Hmask) "HP".
     iPoseProof (ainv_tok_acc with "HP") as "Hinv". eassumption.
@@ -343,8 +295,8 @@ Section inv.
   Qed.
 
   Lemma ainv_tok_acc_iprop {N E} {Px : aProp true} : ↑N ⊆ E →
-    ainv_tok N Px =[inv_wsat ⟦⟧ᶜ]{E,E∖↑N}=∗
-      ▷ Px ∗ (▷ Px =[inv_wsat ⟦⟧ᶜ]{E∖↑N,E}=∗ True).
+    ainv_tok N Px =[inv_wsat]{E,E∖↑N}=∗
+      ▷ Px ∗ (▷ Px =[inv_wsat]{E∖↑N,E}=∗ True).
   Proof.
     iIntros (Hmask) "HP".
     iPoseProof (ainv_tok_acc with "HP") as "Hinv". eassumption.
@@ -352,8 +304,8 @@ Section inv.
   Qed.
 
   Lemma ainv_tok_acc_2 {N1 N2 E} {P : aProp false} : N1 ## N2 -> ↑N2 ⊆ E -> ↑N1 ⊆ E →
-    ainv_tok N2 (ainv_tok N1 P) =[inv_wsat ⟦⟧ᶜ]{E,E∖↑N2∖↑N1}=∗
-      invariant_unfold P ∗ (invariant_unfold P =[inv_wsat ⟦⟧ᶜ]{E∖↑N2∖↑N1,E}=∗ True).
+    ainv_tok N2 (ainv_tok N1 P) =[inv_wsat]{E,E∖↑N2∖↑N1}=∗
+      invariant_unfold P ∗ (invariant_unfold P =[inv_wsat]{E∖↑N2∖↑N1,E}=∗ True).
   Proof.
     simpl.
     iIntros (Hneq HN2 HN1) "Hinv W".
@@ -370,66 +322,43 @@ Section inv.
     by iFrame.
   Qed.
 
-  Lemma inv_iff' {N : namespace} `{!Deriv ih δ} {Px Qx : cif CON Σ} :
-    □ (∀ δ, ⌜Deriv ih δ⌝ -∗ ⟦ Px ⟧(δ) ∗-∗ ⟦ Qx ⟧(δ)) -∗
-    inv' δ N Px -∗ inv' δ N Qx.
-  Proof.
-    iIntros "#Hequiv".
-    iApply inv'_iff.
-    iModIntro. iIntros.
-    by iApply "Hequiv".
-  Qed.
-
-  Lemma inv_iff {N : namespace} `{!Deriv ih δ} {Px Qx : cif CON Σ} :
-    □ (∀ δ, ⌜Deriv ih δ⌝ -∗ ⟦ Px ⟧(δ) ∗-∗ ⟦ Qx ⟧(δ)) -∗
-    inv' δ N Px ∗-∗ inv' δ N Qx.
-  Proof.
-    iIntros "#Hequiv".
-    iSplit; iApply inv_iff'; iIntros "!> %δ' %Hderiv". by iApply "Hequiv".
-    iApply util.wand_iff_comm. by iApply "Hequiv".
-  Qed.
-
   Lemma semantic_alteration_equiv' {b1 b2} N (P : aProp b1) (Q : aProp b2) :
-    □ (P ≡ Q)%a -∗
+    (⊢ (P ≡ Q)%a) ->
     ainv_tok N P -∗ ainv_tok N Q.
   Proof.
-    iIntros "[-> #Hequiv]".
+    unfold aProp_equivalence; intros Hequiv.
     unfold ainv_tok; cbn.
     iIntros "Hinv".
-    iApply (inv'_iff with "[] Hinv").
-    iIntros "!>" (δ' HDeriv _ Hsound).
-    unfold aProp_to_ofe_car.
-    destruct b2; dependent destruction P; dependent destruction Q; cbn.
-    - iSplit; iIntros; iNext; by iApply ("Hequiv" $! δ').
-    - iSplit; cbn; iIntros "HP".
-      + iApply b0. iApply ("Hequiv" $! _ _ HDeriv). by iApply b.
-      + iApply b. iApply ("Hequiv" $! _ _ HDeriv). by iApply b0.
+    dependent destruction P; dependent destruction Q; cbn in *;
+      iApply (inv.sem_alteration with "Hinv"); cbn.
+    - iSplit; iIntros; iNext; by iApply Hequiv.
+    - iApply bi.wand_iff_trans. iSplitL; [iApply b | ].
+      iApply bi.wand_iff_sym. iApply Hequiv.
+    - iApply bi.wand_iff_trans. iSplitL; iApply bi.wand_iff_sym; [ | iApply b ].
+      iApply Hequiv.
+    - iApply bi.wand_iff_trans. iSplitL; [ iApply b0 | ].
+      iApply bi.wand_iff_trans. iSplitL; iApply bi.wand_iff_sym; [ | iApply b ].
+      iApply Hequiv.
   Qed.
 
   Lemma semantic_alteration_equiv {b1 b2} N (P : aProp b1) (Q : aProp b2) :
-    □ (P ≡ Q)%a -∗
+    (⊢ (P ≡ Q)%a) ->
     ainv_tok N P ∗-∗ ainv_tok N Q.
   Proof.
-    iIntros "[-> #Hequiv]".
-    iSplit; iApply semantic_alteration_equiv'; (iSplitR; [ iPureIntro; reflexivity | ]);
-      iIntros "%δ %ih %Hder"; [ | rewrite util.wand_iff_comm ];
-      iApply ("Hequiv" $! _ _ Hder).
+    intros Hequiv.
+    iSplit; iApply semantic_alteration_equiv'.
+    - apply Hequiv.
+    - dependent destruction P; dependent destruction Q; cbn in *;
+      iApply bi.wand_iff_sym; iApply Hequiv.
   Qed.
 
   Lemma semantic_alteration_equiv_equiv {b1 b2} N (P : aProp b1) (Q : aProp b2) :
-    □ (P ≡ Q)%a -∗
-    aProp_equivalence (ainv_tok N P) (ainv_tok N Q).
+    (⊢ (P ≡ Q)%a) ->
+    ⊢ aProp_equivalence (ainv_tok N P) (ainv_tok N Q).
   Proof.
-    iIntros "[-> #Hequiv]"; iSplit; [ iPureIntro; reflexivity | ].
-    iIntros "%δ %ih %Hder".
-    simpl.
-    iApply inv'_iff'; iIntros "%δ' %Hder' _ _ !>".
-    iSpecialize ("Hequiv" $! _ _ Hder').
-    destruct b2; dependent destruction P; dependent destruction Q; cbn.
-    - iSplit; iIntros; iNext; by iApply "Hequiv".
-    - iSplit; iIntros "HP".
-      + iApply b0. iApply ("Hequiv"). by iApply b.
-      + iApply b. iApply ("Hequiv"). by iApply b0.
+    intros Hequiv.
+    destruct b2; dependent destruction P; dependent destruction Q;
+      iApply semantic_alteration_equiv; apply Hequiv.
   Qed.
 
   Lemma exist_intro {A : Type} {b} {Ψ : A → aProp b} (a : A) : Ψ a ⊢ (∃ a0 : A, Ψ a0)%a.
@@ -445,62 +374,36 @@ Section inv.
     ((∃ a, P a) ≡ (∃ a, Q a))%a.
   Proof.
     iIntros "Hequiv".
-    iSplit; [iPureIntro; reflexivity | ]; iIntros "% % %Hder".
-    iSplit; (destruct b; cbn;  iIntros "[%a HP]"; iExists a;
-      iDestruct ("Hequiv" $! a) as "[_ Hequiv]";
-      [ by iApply ("Hequiv" $! _ _ der_Deriv)
-      | by iApply ("Hequiv" $! _ _ Hder) ]).
+    destruct b; cbn in *;
+      iSplit; iIntros "[%a HP]"; iExists a;
+      iSpecialize ("Hequiv" $! a);
+      remember (P a) as Pa; remember (Q a) as Qa;
+      dependent destruction Pa; dependent destruction Qa;
+      by iApply "Hequiv".
   Qed.
 
   Lemma aProp_equiv_sep_comm {b₁ b₂} (P : aProp b₁) (Q : aProp b₂):
     ⊢ ((P ∗ Q)%a ≡ (Q ∗ P)%a)%a.
   Proof.
-    iSplit; [iPureIntro; apply orb_comm | ]; iIntros "% % %HdePr".
-    dependent destruction P;  dependent destruction Q; cbn;
-      rewrite bi.sep_comm; iApply bi.wand_iff_refl.
+    dependent destruction P; dependent destruction Q; cbn;
+    rewrite bi.sep_comm; iApply bi.wand_iff_refl.
   Qed.
 
   Lemma aProp_equiv_IProp (P Q : aProp true) :
     P ∗-∗ Q -∗
     (P ≡ Q)%a.
   Proof.
-    iIntros "Hequiv".
-    iSplit; [iPureIntro; reflexivity | ]; iIntros "% % %Hder".
-    dependent destruction P;  dependent destruction Q; cbn; done.
-  Qed.
-
-  Lemma aProp_equiv_notderiv {b} (P Q : aProp b) `{!NotDeriv P, !NotDeriv Q} :
-    P ∗-∗ Q -∗
-    (P ≡ Q)%a.
-  Proof.
-    iIntros "Hequiv".
-    iSplit; [iPureIntro; reflexivity | ]; iIntros "% % %Hder".
-    dependent destruction P;  dependent destruction Q; cbn; first done.
-    destruct NotDeriv0 as [[Qp HP]].
-    destruct NotDeriv1 as [[Qq HQ]].
-    iSplit; iIntros "HP".
-    - iApply HQ. iPoseProof (HP with "HP") as "HP".
-      iApply (HQ der). iApply "Hequiv". by iApply HP.
-    - iApply HP. iPoseProof (HQ with "HP") as "HQ".
-      iApply (HP der). iApply "Hequiv". by iApply HQ.
+    iIntros "Hequiv";
+    dependent destruction P; dependent destruction Q; cbn;
+    iApply "Hequiv".
   Qed.
 
   Lemma commute_under_inv {b} N₁ N₂ (P : aProp b) (Q : aProp b) :
     ainv_tok N₁ (ainv_tok N₂ (P ∗ Q)) ∗-∗ ainv_tok N₁ (ainv_tok N₂ (Q ∗ P)).
   Proof.
-    iApply semantic_alteration_equiv; iIntros "!>".
-    iApply semantic_alteration_equiv_equiv; iIntros "!>".
+    iApply semantic_alteration_equiv.
+    iApply semantic_alteration_equiv_equiv.
     iApply aProp_equiv_sep_comm.
-  Qed.
-
-  Lemma commute_under_inv_notderiv {b} N₁ N₂ (P Q : aProp b) `{!NotDeriv P, !NotDeriv Q} :
-    ainv_tok N₁ (ainv_tok N₂ (P ∗ Q)) ∗-∗ ainv_tok N₁ (ainv_tok N₂ (Q ∗ P)).
-  Proof.
-    iApply semantic_alteration_equiv; iIntros "!>".
-    iApply semantic_alteration_equiv_equiv; iIntros "!>".
-    iApply aProp_equiv_notderiv.
-    dependent destruction P; dependent destruction Q; cbn;
-      rewrite bi.sep_comm; iApply bi.wand_iff_refl.
   Qed.
 
   Lemma modus_aponens {b1 b2} (P : aProp b1) (Q : aProp b2) :
