nola/iris/dinv.v
@@ -1,29 +1,32 @@
 (** * Direct invariants *)
 
 From nola.bi Require Export internal modw.
+From nola.iris Require Export cif.
 From nola.iris Require Export iprop.
 From nola.iris Require Import sinv.
 From iris.proofmode Require Import proofmode.
 Import iPropAppNotation ModwNotation.
 
-Implicit Type (FML : oFunctor) (i : positive).
+Implicit Type (i : positive).
 
 (** Ghost state for direct invariants *)
-Class dinvGpreS FML Σ : Type := dinvGpreS_sinv : sinvGpreS FML Σ.
+Class dinvGpreS Σ : Type := dinvGpreS_sinv : sinvGpreS Σ.
 Local Existing Instance dinvGpreS_sinv.
-Class dinvGS FML Σ : Type := dinvGS_sinv : sinvGS FML Σ.
+Class dinvGS Σ : Type := dinvGS_sinv : sinvGS Σ.
 Local Existing Instance dinvGS_sinv.
-Definition dinvΣ FML `{!oFunctorContractive FML} := sinvΣ FML.
+Definition dinvΣ:= sinvΣ.
 #[export] Instance subG_dinvΣ
-  `{!oFunctorContractive FML, !subG (dinvΣ FML) Σ} : dinvGpreS FML Σ.
+  `{!subG (dinvΣ Σ) Σ} : dinvGpreS Σ.
 Proof. solve_inG. Qed.
 
 Section dinv.
-  Context `{!dinvGS FML Σ}.
-  Implicit Type Px : FML $oi Σ.
+  Context `{!dinvGS Σ}.
+  Context `{!Csem CON JUDG Σ, !Jsem JUDG (iProp Σ)}.
+  Implicit Type Px : cif CON Σ.
+  Import CsemNotation.
 
   (** [dinv_tok]: Direct invariant token *)
-  Local Definition dinv_tok_def (Px : FML $oi Σ) : iProp Σ :=
+  Local Definition dinv_tok_def (Px : cif CON Σ) : iProp Σ :=
     ∃ i, sinv_tok i Px.
   Local Definition dinv_tok_aux : seal dinv_tok_def. Proof. by eexists. Qed.
   Definition dinv_tok := dinv_tok_aux.(unseal).
@@ -39,11 +42,11 @@ Section dinv.
   #[export] Instance dinv_tok_persistent {Px} : Persistent (dinv_tok Px).
   Proof. rewrite dinv_tok_unseal. exact _. Qed.
   (** [dinv_tok] is timeless for discrete formulas *)
-  #[export] Instance dinv_tok_timeless `{!Discrete Px} : Timeless (dinv_tok Px).
+  #[export] Instance dinv_tok_timeless `{!Discrete ⟦Px⟧ᶜ} : Timeless (dinv_tok Px).
   Proof. rewrite dinv_tok_unseal. exact _. Qed.
 
   (** World satisfaction *)
-  Local Definition dinv_wsat_def (sm : FML $oi Σ -d> iProp Σ) : iProp Σ :=
+  Local Definition dinv_wsat_def (sm : iProp Σ -d> iProp Σ) : iProp Σ :=
     sinv_wsat (λ _, sm).
   Local Definition dinv_wsat_aux : seal dinv_wsat_def. Proof. by eexists. Qed.
   Definition dinv_wsat := dinv_wsat_aux.(unseal).
@@ -56,16 +59,9 @@ Section dinv.
   #[export] Instance dinv_wsat_proper : Proper ((≡) ==> (≡)) dinv_wsat.
   Proof. apply ne_proper, _. Qed.
 
-  (** [dinv_wsat] is timeless if [sm] is always timeless
-    and the underlying ofe is discrete *)
-  #[export] Instance dinv_wsat_timeless
-    `{!OfeDiscrete (FML $oi Σ), !∀ Px, Timeless (sm Px)} :
-    Timeless (dinv_wsat sm).
-  Proof. rewrite dinv_wsat_unseal. exact _. Qed.
-
   (** Allocate [dinv_tok] suspending the world satisfaction *)
   Lemma dinv_tok_alloc_suspend {sm} Px :
-    dinv_wsat sm ==∗ dinv_tok Px ∗ (sm Px -∗ dinv_wsat sm).
+    dinv_wsat sm ==∗ dinv_tok Px ∗ (sm ⟦Px⟧ᶜ -∗ dinv_wsat sm).
   Proof.
     rewrite dinv_tok_unseal dinv_wsat_unseal. iIntros "W".
     iDestruct (sinv_tok_alloc_suspend Px with "W") as (I) "big".
@@ -73,7 +69,7 @@ Section dinv.
     iModIntro. iFrame "inv". iIntros "?". by iApply "→W".
   Qed.
   (** Allocate [dinv_tok] *)
-  Lemma dinv_tok_alloc {sm} Px : sm Px =[dinv_wsat sm]=∗ dinv_tok Px.
+  Lemma dinv_tok_alloc {sm} Px : sm ⟦Px⟧ᶜ =[dinv_wsat sm]=∗ dinv_tok Px.
   Proof.
     iIntros "? W". iMod (dinv_tok_alloc_suspend with "W") as "[$ →W]".
     iModIntro. by iApply "→W".
@@ -81,14 +77,14 @@ Section dinv.
 
   (** Access the content of [dinv_tok] *)
   Lemma dinv_tok_acc {sm Px} :
-    dinv_tok Px -∗ dinv_wsat sm -∗ sm Px ∗ (sm Px -∗ dinv_wsat sm).
+    dinv_tok Px -∗ dinv_wsat sm -∗ sm ⟦Px⟧ᶜ ∗ (sm ⟦Px⟧ᶜ -∗ dinv_wsat sm).
   Proof.
     rewrite dinv_tok_unseal dinv_wsat_unseal. iIntros "[% i] W".
     iDestruct (sinv_tok_acc with "i W") as "[$$]".
   Qed.
   (** Access the content of [dinv_tok] for persistent propositions *)
-  Lemma dinv_tok_acc_persistent {sm Px} : Persistent (sm Px) →
-    dinv_tok Px -∗[dinv_wsat sm] sm Px.
+  Lemma dinv_tok_acc_persistent {sm Px} : Persistent (sm ⟦Px⟧ᶜ) →
+    dinv_tok Px -∗[dinv_wsat sm] sm ⟦Px⟧ᶜ.
   Proof.
     iIntros (?) "i W". iDestruct (dinv_tok_acc with "i W") as "[#Px cl]".
     iFrame "Px". by iApply "cl".
@@ -96,8 +92,8 @@ Section dinv.
 End dinv.
 
 (** Allocate [dinv_wsat] *)
-Lemma dinv_wsat_alloc `{!dinvGpreS FML Σ} :
-  ⊢ |==> ∃ _ : dinvGS FML Σ, ∀ sm, internal_ne sm -∗ dinv_wsat sm.
+Lemma dinv_wsat_alloc `{!dinvGpreS Σ} :
+  ⊢ |==> ∃ _ : dinvGS Σ, ∀ sm, internal_ne sm -∗ dinv_wsat sm.
 Proof.
   iMod sinv_wsat_alloc as (γ) "W". iModIntro. iExists _. iIntros (?) "Ne".
   rewrite dinv_wsat_unseal. iApply "W". by iIntros.
