nola/iris/sinv.v
@@ -1,37 +1,39 @@
 (** * Simple invariants *)
 
-From nola.bi Require Export internal modw.
+From nola.bi Require Export internal modw deriv.
 From nola.iris Require Export iprop.
 From iris.algebra Require Import agree gmap_view.
-From iris.base_logic.lib Require Export own.
+From iris.base_logic.lib Require Export own wsat invariants.
+From iris.algebra Require Import gset.
 From iris.proofmode Require Import proofmode.
+From nola.iris Require Export cif.
 Import iPropAppNotation.
 
-Implicit Type FML : oFunctor.
-
 (** Ghost state for simple invariants *)
-Class sinvGpreS FML Σ : Type :=
-  sinvGpreS_in : inG Σ (gmap_viewR positive (agreeR (FML $oi Σ))).
+Class sinvGpreS Σ : Type :=
+  sinvGpreS_in : inG Σ (gmap_viewR positive (agreeR (iProp Σ))).
 Local Existing Instance sinvGpreS_in.
-Class sinvGS FML Σ : Type := SinvGS {
-  sinvGS_pre : sinvGpreS FML Σ;
+Class sinvGS Σ : Type := SinvGS {
+  sinvGS_pre : sinvGpreS Σ;
   sinv_name : gname;
 }.
 Local Existing Instance sinvGS_pre.
-Definition sinvΣ FML `{!oFunctorContractive FML} : gFunctors :=
-  GFunctor (gmap_viewRF positive (agreeRF FML)).
+Definition sinvΣ Σ : gFunctors :=
+  GFunctor (gmap_viewRF positive (agreeRF (iPropO Σ))).
 #[export] Instance subG_sinvΣ
-  `{!oFunctorContractive FML, !subG (sinvΣ FML) Σ} : sinvGpreS FML Σ.
+  `{!subG (sinvΣ Σ) Σ} : sinvGpreS Σ.
 Proof. solve_inG. Qed.
 
 Section sinv.
-  Context `{!sinvGS FML Σ}.
-  Implicit Type (Px : FML $oi Σ) (sm : positive → FML $oi Σ → iProp Σ)
+  Context `{!sinvGS Σ, !invGS_gen hlc Σ, !Csem CON JUDG Σ, !Jsem JUDG (iProp Σ)}.
+  Implicit Type (Px : cif CON Σ) (sm : positive → iProp Σ → iProp Σ)
     (i : positive).
+
+  Import CsemNotation.
 
   (** Simple invariant token *)
   Local Definition sinv_tok_def i Px : iProp Σ :=
-    own sinv_name (gmap_view_frag i DfracDiscarded (to_agree Px)).
+    own sinv_name (gmap_view_frag i DfracDiscarded (to_agree ⟦ Px ⟧ᶜ)).
   Local Lemma sinv_tok_aux : seal sinv_tok_def. Proof. by eexists. Qed.
   Definition sinv_tok := sinv_tok_aux.(unseal).
   Local Lemma sinv_tok_unseal : sinv_tok = sinv_tok_def.
@@ -39,11 +41,11 @@ Section sinv.
 
   (** Authoritative token *)
   Local Definition sinv_auth_tok M :=
-    own sinv_name (gmap_view_auth (DfracOwn 1) (to_agree <$> M)).
+    own sinv_name (gmap_view_auth (DfracOwn 1) (to_agree <$> M)). About sinv_auth_tok.
   (** World satisfaction *)
   Definition sinv_wsat_def sm : iProp Σ :=
     (∀ i, internal_ne (sm i)) ∗
-    ∃ M, sinv_auth_tok M ∗ [∗ map] i ↦ Px ∈ M, sm i Px.
+    ∃ M, sinv_auth_tok M ∗ [∗ map] i ↦ P ∈ M, sm i P.
   Local Lemma sinv_wsat_aux : seal sinv_wsat_def. Proof. by eexists. Qed.
   Definition sinv_wsat := sinv_wsat_aux.(unseal).
   Local Lemma sinv_wsat_unseal : sinv_wsat = sinv_wsat_def.
@@ -58,7 +60,7 @@ Section sinv.
   #[export] Instance sinv_tok_persistent {i Px} : Persistent (sinv_tok i Px).
   Proof. rewrite sinv_tok_unseal. exact _. Qed.
   (** [sinv_tok] is timeless for discrete formulas *)
-  #[export] Instance sinv_tok_timeless `{!Discrete Px} {i} :
+  #[export] Instance sinv_tok_timeless `{!Discrete ⟦Px⟧ᶜ} {i} :
     Timeless (sinv_tok i Px).
   Proof. rewrite sinv_tok_unseal /sinv_tok_def /gmap_view_frag. exact _. Qed.
 
@@ -76,25 +78,19 @@ Section sinv.
     rewrite sinv_wsat_unseal /sinv_wsat_def=> ?? eqv. repeat f_equiv. apply eqv.
   Qed.
 
-  (** [sinv_wsat] is timeless if [sm] is always timeless
-    and the underlying ofe is discrete *)
-  #[export] Instance sinv_wsat_timeless
-    `{!OfeDiscrete (FML $oi Σ), !∀ i Px, Timeless (sm i Px)} :
-    Timeless (sinv_wsat sm).
-  Proof. rewrite sinv_wsat_unseal. exact _. Qed.
-
   (** Lemma for [sinv_tok_alloc_suspend] *)
   Local Lemma sinv_auth_tok_alloc {M i Px} : i ∉ dom M →
-    sinv_auth_tok M ==∗ sinv_auth_tok (<[i:=Px]> M) ∗ sinv_tok i Px.
+    sinv_auth_tok M ==∗ sinv_auth_tok (<[i:=⟦ Px ⟧ᶜ]> M) ∗ sinv_tok i Px.
   Proof.
     move=> /not_elem_of_dom eq. iIntros "●". rewrite sinv_tok_unseal -own_op.
     iApply own_update; [|done]. rewrite fmap_insert.
     apply gmap_view_alloc; [|done..]. by rewrite lookup_fmap eq.
   Qed.
+
   (** Allocate [sinv_tok] suspending the world satisfaction *)
   Lemma sinv_tok_alloc_suspend {sm} Px :
     sinv_wsat sm -∗ ∃ I : gset positive, ∀ i, ⌜i ∉ I⌝ ==∗
-      sinv_tok i Px ∗ (sm i Px -∗ sinv_wsat sm).
+      sinv_tok i Px ∗ (sm i ⟦Px⟧ᶜ -∗ sinv_wsat sm).
   Proof.
     rewrite sinv_wsat_unseal. iIntros "[Ne[%M[● M]]]". iExists (dom M).
     iIntros (i ?). iMod (sinv_auth_tok_alloc with "●") as "[● #i]"; [done|].
@@ -104,7 +100,7 @@ Section sinv.
 
   (** Lemma for [sinv_tok_acc] *)
   Local Lemma sinv_auth_tok_lookup {M i Px} :
-    sinv_auth_tok M -∗ sinv_tok i Px -∗ ∃ Px', ⌜M !! i = Some Px'⌝ ∧ Px ≡ Px'.
+    sinv_auth_tok M -∗ sinv_tok i Px -∗ ∃ (Px' : iProp Σ), ⌜M !! i = Some Px'⌝ ∧ ⟦ Px ⟧ᶜ ≡ Px'.
   Proof.
     rewrite sinv_tok_unseal. iIntros "● i".
     iDestruct (own_valid_2 with "● i") as "✓".
@@ -114,7 +110,7 @@ Section sinv.
   Qed.
   (** Access via [sinv_tok] *)
   Lemma sinv_tok_acc {i sm Px} :
-    sinv_tok i Px -∗ sinv_wsat sm -∗ sm i Px ∗ (sm i Px -∗ sinv_wsat sm).
+    sinv_tok i Px -∗ sinv_wsat sm -∗ sm i ⟦Px⟧ᶜ ∗ (sm i ⟦Px⟧ᶜ -∗ sinv_wsat sm).
   Proof.
     rewrite sinv_wsat_unseal. iIntros "i [#Ne[%M[● M]]]".
     iDestruct (sinv_auth_tok_lookup with "● i") as (Px' eq) "#≡".
@@ -122,18 +118,32 @@ Section sinv.
     iDestruct (big_sepM_lookup_acc with "M") as "[$ →M]"; [done|]. iIntros "Px".
     iFrame "Ne ●". by iApply "→M".
   Qed.
+
+  Lemma sem_alteration {i Px Qx} :
+    (⟦ Px ⟧ᶜ ∗-∗ ⟦ Qx ⟧ᶜ) ->
+    sinv_tok i Px ∗-∗ sinv_tok i Qx.
+  Proof.
+    intros Heq.
+    iSplit; iIntros "Hinv"; rewrite sinv_tok_unseal /sinv_tok_def.
+    - iApply (own_mono with "Hinv").
+      exists ε. rewrite ucmra_unit_right_id.
+      f_equiv. f_equiv. apply bi.wand_iff_equiv. apply Heq.
+    - iApply (own_mono with "Hinv").
+      exists ε. rewrite ucmra_unit_right_id.
+      f_equiv. f_equiv. symmetry. apply bi.wand_iff_equiv. apply Heq.
+  Qed.
 End sinv.
 
 (** Lemma for [sinv_wsat_alloc] *)
-Local Lemma sinv_auth_tok_alloc_empty `{!sinvGpreS FML Σ} :
-  ⊢ |==> ∃ _ : sinvGS FML Σ, sinv_auth_tok ∅.
+Local Lemma sinv_auth_tok_alloc_empty `{!sinvGpreS Σ} :
+  ⊢ |==> ∃ _ : sinvGS Σ, sinv_auth_tok ∅.
 Proof.
   iMod (own_alloc (gmap_view_auth (DfracOwn 1) ∅)) as (γ) "●".
-  { apply gmap_view_auth_valid. } { iModIntro. by iExists (SinvGS _ _ _ γ). }
+  { apply gmap_view_auth_valid. } { iModIntro. by iExists (SinvGS _ _ γ). }
 Qed.
 (** Allocate [sinv_wsat] *)
-Lemma sinv_wsat_alloc `{!sinvGpreS FML Σ} :
-  ⊢ |==> ∃ _ : sinvGS FML Σ, ∀ sm, (∀ i, internal_ne (sm i)) -∗ sinv_wsat sm.
+Lemma sinv_wsat_alloc `{!sinvGpreS Σ} :
+  ⊢ |==> ∃ _ : sinvGS Σ, ∀ sm, (∀ i, internal_ne (sm i)) -∗ sinv_wsat sm.
 Proof.
   iMod sinv_auth_tok_alloc_empty as (?) "●". iModIntro. iExists _.
   iIntros (?) "Ne". rewrite sinv_wsat_unseal. by iFrame.
