nola/iris/dinv_deriv.v
@@ -45,7 +45,7 @@ End dinvJ.
 Notation dinvd := (dinv der).
 
 Section dinvJ.
-  Context `{!dinvGS FML Σ, !dinvJ (FML $oi Σ) JUDG,
+  Context `{!dinvGS Σ, !dinvJ (FML $oi Σ) JUDG,
     !Dsem JUDG (FML $oi Σ) (iProp Σ)}.
   Implicit Type δ : JUDG -n> iProp Σ.
 
